compose plays

models/Play.v
@@ -1,116 +1,120 @@
 Require Import structures.Effects.
+Require Import Poset.
+Require Import Downset.
+From structures Require Import Lattice.
+From lattices Require Import LatticeProduct.
 
 Set Asymmetric Patterns.
 
-(* Inductive play {E F: esig} (A: Type) : Type := *)
-(* | pr: A -> play A *)
-(* | prq {A'}: A -> F A' -> play A' -> play A *)
-(* | pm {B}: E B -> play A *)
-(* | pmn {B}: E B -> B -> play A -> play A. *)
-
-Inductive play {E : esig} {V: Type} :=
-| pret: V -> play
-| pmove: forall {X}, E X -> play
-| pcons: forall {X}, E X -> X -> play -> play.
-Arguments play: clear implicits.
-
-Inductive plays {E F : esig} :=
-| pnil: plays
-| prun: forall {X}, F X -> play E (X * plays) -> plays.
-Arguments plays: clear implicits.
-
-Require Import Poset.
-
-Module Downset.
-  Record downset {C : poset} :=
-    {
-      has : C -> Prop;
-      closed x y : x [= y -> has y -> has x;
-    }.
-
-  Arguments downset : clear implicits.
-
-  Program Definition emb {C : poset} (c : C) : downset C :=
-    {|
-      has x := ref x c;
-    |}.
-  Next Obligation. etransitivity; eauto. Qed.
-End Downset.
-
-Inductive plays_ref {E F} : plays E F -> plays E F -> Prop := .
-Program Definition plays_poset E F : poset :=
-  {|
-    poset_carrier := plays E F;
-    ref := plays_ref;
-  |}.
-Next Obligation. Admitted.
-Next Obligation. Admitted.
-
-Definition s E F := Downset.downset (plays_poset E F).
-
-Definition events (E: esig) := @play E unit.
-
-Inductive run_play {E X}: play E X -> events E -> option X -> Prop :=
-| run_pret v : run_play (pret v) (pret tt) (Some v)
-| run_pmove {X_m} (m: E X_m) : run_play (pmove m) (pmove m) None
-| run_pcons {X'} (m: E X') n p e (v: option X):
-  run_play p e v ->
-  run_play (pcons m n p) (pcons m n e) v.
-
-Inductive concat_events {E}: events E -> events E -> events E -> Prop :=
-| concat_pret e: concat_events (pret tt) e e
-| concat_pmove {X} (m: E X) e: concat_events (pmove m) e (pmove m)
-| concat_pcons {X} (m: E X) n e1 e2 e:
-  concat_events e1 e2 e -> concat_events (pcons m n e1) e2 (pcons m n e).
-
-Inductive run_plays {E F}: plays E F -> events F -> events E -> option (plays E F) -> Prop :=
-| runs_nil st: run_plays st (pret tt) (pret tt) (Some st)
-| runs_cons' {X} (m_f: F X) play_e es res:
-  run_play play_e es res -> run_plays (prun m_f play_e) (pmove m_f) es None
-| runs_cons {X} (m_f: F X) n_f play_e st_ef st_ef' es_e1 es_e2 es_e es_f:
-  run_play play_e es_e1 (Some (n_f, st_ef)) ->
-  run_plays st_ef es_f es_e2 st_ef' ->
-  concat_events es_e1 es_e2 es_e ->
-  run_plays (prun m_f play_e) (pcons m_f n_f es_f) es_e st_ef'.
-
-Inductive compose_plays {E F G}: plays F G -> plays E F -> plays E G -> Prop :=
-| compose_nil st: compose_plays pnil st pnil
-| compose_prun {X} play_e play_f es_f es_e (m_g: G X) n_g st_fg' st_ef st_ef' st_eg':
-  compose_plays st_fg' st_ef' st_eg' ->
-  run_play play_f es_f (Some (n_g, st_fg')) ->
-  run_plays st_ef es_f es_e (Some st_ef') ->
-  run_play play_e es_e (Some (n_g, st_eg')) ->
-  compose_plays (prun m_g play_f) st_ef (prun m_g play_e)
-| compose_prun_none {X} play_e play_f es_f es_e (m_g: G X) st_ef res:
-  run_play play_f es_f None ->
-  run_plays st_ef es_f es_e res ->
-  run_play play_e es_e None ->
-  compose_plays (prun m_g play_f) st_ef (prun m_g play_e)
-| compose_prun_none' {X} play_e play_f es_f es_e (m_g: G X) st_ef res:
-  run_play play_f es_f res ->
-  run_plays st_ef es_f es_e None ->
-  run_play play_e es_e None ->
-  compose_plays (prun m_g play_f) st_ef (prun m_g play_e).
-
-Include Downset.
-
-Inductive id_plays {E}: plays E E -> Prop := 
-| id_plays_intro {X} (m: E X) n s:
-  id_plays s -> id_plays (prun m (pcons m n (pret (n, s)))).
-
-Program Definition id {E}: s E E :=
-  {| has p := id_plays p |}.
-Next Obligation. Admitted.
-
-Program Definition compose {E F G} (s1: s F G) (s2: s E F): s E G :=
-  {|
-    has p := exists p1 p2, has s1 p1 /\ has s2 p2 /\ compose_plays p1 p2 p;
-  |}.
-Next Obligation. Admitted.
-
-Lemma s_ext {E F} (s1 s2: s E F): (forall p, has s1 p <-> has s2 p) -> s1 = s2.
+Lemma bot_elim {C: poset} (t: C):
+  down t [= bot -> False.
 Proof.
+  Local Transparent bot. unfold bot.
+  intros H. apply Downset.emb_join_prime in H.
+  destruct H as ([] & _).
+Qed.
+
+Lemma fsup_mor {L M: cdlattice} {f: L -> M} `{Sup.Morphism _ _ f}:
+  forall {I} (P : I -> Prop) (M: I -> L), f (sup {x | P x}, M x) = sup {x | P x}, f (M x).
+Proof. intros. unfold fsup. eapply Sup.mor. Qed.
+
+Inductive play {E F: esig} (A: Type) : Type :=
+| pr: A -> play A
+| prq {A'}: A -> F A' -> play A' -> play A
+| pm {B}: E B -> play A
+| pmn {B}: E B -> B -> play A -> play A.
+Arguments play: clear implicits.
+Arguments pr {E F A} r.
+Arguments prq {E F A A'} r q next.
+Arguments pm {E F A B} m.
+Arguments pmn {E F A B} m n next.
+
+Inductive play_ref {E F A} : play E F A -> play E F A -> Prop :=
+| play_ref_pr1 r:
+  play_ref (pr r) (pr r)
+| play_ref_pr2 {A'} r (q: F A') next:
+  play_ref (pr r) (prq r q next)
+| play_ref_prq {A'} r (q: F A') next next':
+  play_ref next next' ->
+  play_ref (prq r q next) (prq r q next')
+| play_ref_pm1 {B} (m: E B):
+  play_ref (pm m) (pm m)
+| play_ref_pm2 {B} (m: E B) n next:
+  play_ref (pm m) (pmn m n next)
+| play_ref_pmn {B} (m: E B) n next next':
+  play_ref next next' ->
+  play_ref (pmn m n next) (pmn m n next').
+
+Lemma play_ref_preo {E F A}: PreOrder (@play_ref E F A).
 Admitted.
+
+Lemma play_ref_antisym {E F A}: Antisymmetric _ eq (@play_ref E F A).
+Admitted.
+
+Canonical Structure play_poset E F A : poset :=
+  {|
+    poset_carrier := play E F A;
+    ref := play_ref;
+    ref_preo := play_ref_preo;
+    ref_po := play_ref_antisym;
+  |}.
+
+Definition t E F A : cdlattice := downset (play_poset E F A).
+
+Definition s (E F : esig) : cdlattice := pi A, t E F A ^ F A.
+
+Definition initial_state {E F A} (s: s E F) (q: F A): t E F A := s _ q.
+Definition at_external {E F A B} (p: t E F A) (m: E B): Prop :=
+  down (pm m) [= p.
+Definition after_external {E F A B} (p: t E F A) (m: E B) (n: B): t E F A :=
+  sup {p' | down (pmn m n p') [= p}, down p'.
+Definition at_final {E F A} (p: t E F A) (r: A): Prop :=
+  down (pr r) [= p.
+Definition after_final {E F A A'} (p: t E F A) (r: A) (q: F A'): t E F A' :=
+  sup {p' | down (prq r q p') [= p}, down p'.
+
+Program Fixpoint compose_play2  {E F G A B} (k: B -> s E F -> t E G A) (t2: play E F B): t E G A :=
+  match t2 with
+  | pm _ m => down (pm m)
+  | pmn _ m n p_next =>
+      Downset.map (fun p => pmn m n p) (compose_play2 k p_next)
+  | pr r => k r (fun _ _ => bot)
+  | prq A r q p_next =>
+      k r (fun A' q' => _)
+  end.
+Next Obligation.
+  refine (sup HA: A = A', _). subst A'.
+  refine (sup H: q = q', down p_next).
+Defined.
+
+Definition compose_t2 {E F G A B} (k: B -> s E F -> t E G A) (t2: t E F B): t E G A :=
+  Downset.ext (compose_play2 k) t2.
+
+Fixpoint compose_play1 {E F G A} (s2: s E F) (p1: play F G A): t E G A :=
+  match p1 with
+  | pr r => down (pr r)
+  | prq _ r q p_next =>
+      Downset.map (fun p => prq r q p) (compose_play1 s2 p_next)
+  | pm _ m => compose_t2 (fun _ _ => bot) (s2 _ m)
+  | pmn _ m n p_next =>
+      compose_t2 (fun n' t2' => sup H : n' = n, compose_play1 t2' p_next) (s2 _ m)
+  end.
+
+Definition compose_t1 {E F G A} (t1: t F G A) (t2: s E F): t E G A :=
+  Downset.ext (compose_play1 t2) t1.
+
+Definition compose {E F G} (s1: s F G) (s2: s E F): s E G :=
+  fun A q => compose_t1 (s1 _ q) s2.
+
+Inductive id_play {E A} : E A -> play E E A -> Prop :=
+| id_play_intro m m' n p:
+  id_play m' p ->
+  id_play m (pmn m n (prq n m' p)).
+
+Definition id_t {E A} (q: E A): t E E A :=
+  sup p, sup H: id_play q p, down p.
+
+Definition id {E}: s E E := fun A q => id_t q.
 
 From compcert Require Import Coqlib.
 Require Import Classical_Prop.
@@ -123,25 +127,14 @@ Ltac subst_dep :=
   | _ => idtac
   end.
 
-Lemma plays_left_unit1 {E F} pid (pa: plays E F) pb:
-  id_plays pid ->
-  compose_plays pid pa pb ->
-  pa = pb.
-Proof.
-  intros Hid Hp. revert pa pb Hp. induction Hid.
-  intros. inv Hp.
-  - subst_dep. inv H3.
-    subst_dep. inv H6.
-    subst_dep. f_equal.
-    inv H9. specialize (IHHid _ _ H2). subst.
-    inv H11.
-Admitted.
-
 Lemma left_unit {E F} (t: s E F): compose id t = t.
 Proof.
-  apply s_ext. intros p. split.
-  - intros (p1 & p2 & Hp1 & Hp2 & Hpp).
-    cbn in Hp1.
+  apply antisymmetry.
+  - unfold compose, id. intros A q.
+    unfold compose_t1. unfold id_t.
+    rewrite Sup.mor. apply sup_iff. intros p.
+    rewrite Sup.mor. apply sup_iff. intros H.
+    rewrite @Downset.ext_ana. 2: admit.
 Admitted.
 
 Inductive refconv_play {E F} :=
@@ -159,86 +152,520 @@ Inductive refconv_ref {E F} : refconv_play E F -> refconv_play E F -> Prop :=
   refconv_ref s1 s2 ->
   refconv_ref (refconv_cons m1 m2 n1 n2 s1) (refconv_cons m1 m2 n1 n2 s2).
 
-Program Definition refconv_poset E F : poset :=
+
+Lemma refconv_ref_preo {E F}: PreOrder (@refconv_ref E F).
+Admitted.
+
+Lemma refconv_ref_antisym {E F}: Antisymmetric _ eq (@refconv_ref E F).
+Admitted.
+
+Canonical Structure refconv_poset E F : poset :=
   {|
     poset_carrier := refconv_play E F;
     ref := refconv_ref;
+    ref_preo := refconv_ref_preo;
+    ref_po := refconv_ref_antisym;
   |}.
-Next Obligation. Admitted.
-Next Obligation. Admitted.
 
 Definition r E F := downset (refconv_poset E F).
 
-Inductive refconv_play_next {E F X Y} (m1: E X) (m2: F Y) (n1: X) (n2: Y):
-                             refconv_play E F -> refconv_play E F -> Prop :=
-| refconv_play_next_intro s:
-  refconv_play_next m1 m2 n1 n2 (refconv_cons m1 m2 n1 n2 s) s.
-
-Program Definition r_next {E F} (rc: r E F)
-  {X Y} (m1: E X) (m2: F Y) (n1: X) (n2: Y): r E F :=
-  {| has p := exists p', has rc p' /\ refconv_play_next m1 m2 n1 n2 p' p |}.
-Next Obligation. Admitted.
-
 Definition match_ques {E F X Y} (rc: r E F) (m1: E X) (m2: F Y) :=
-  has rc (refconv_ques m1 m2).
+  down (refconv_ques m1 m2) [= rc.
 
 Definition match_answ {E F X Y} (rc: r E F)
   (m1: E X) (m2: F Y) (n1: X) (n2: Y) :=
-  not (has rc (refconv_answ m1 m2 n1 n2)).
+  not (down (refconv_answ m1 m2 n1 n2) [= rc).
 
-Definition p X E F := play E (X * plays E F) -> Prop.
-
-Definition initial_state {E F X} (t: s E F) (m: F X) (p: p X E F): Prop :=
-  forall p', p p' -> has t (prun m p').
-Definition at_external {E F X Y} (p: p X E F) (m: E Y): Prop := p (pmove m).
-Definition after_external {E F X Y} (p1: p X E F) (m: E Y) (n: Y) (p2: p X E F): Prop :=
-  forall p, p2 p -> p1 (pcons m n p).
-Definition final_state {E F X} (p: p X E F) (r: X) (s: s E F): Prop :=
-  forall p', has s p' -> p (pret (r, p')).
+Program Definition r_next {E F} (rc: r E F)
+  {X Y} (m1: E X) (m2: F Y) (n1: X) (n2: Y): r E F :=
+  sup s, sup H: down (refconv_cons m1 m2 n1 n2 s) [= rc, down s.
 
 Section SIM.
   Context {E1 E2 F1 F2: esig}.
 
-  Inductive sim_p {X1 X2} (q1: F1 X1) (q2: F2 X2) (rf: r F1 F2)
-    (sim_s: r E1 E2 -> r F1 F2 -> s E1 F1 -> s E2 F2 -> Prop):
-    r E1 E2 -> p X1 E1 F1 -> p X2 E2 F2 -> Prop :=
-  | sim_p_intro re p1 p2
-      (match_final:
-        forall r1 s1, final_state p1 r1 s1 ->
-        exists r2 s2, final_state p2 r2 s2 /\ match_answ rf q1 q2 r1 r2 /\
-        sim_s re rf s1 s2)
-      (match_external:
-        forall {Y1} (m1: E1 Y1), at_external p1 m1 ->
-        exists {Y2} (m2: E2 Y2), at_external p2 m2 /\ match_ques re m1 m2 /\
-        forall n1 n2, match_answ re m1 m2 n1 n2 ->
-        forall p1', after_external p1 m1 n1 p1' ->
-        exists p2', after_external p2 m2 n2 p2' /\
-        sim_p q1 q2 rf sim_s (r_next re m1 m2 n1 n2) p1' p2'):
-    sim_p q1 q2 rf sim_s re p1 p2.
+  Fixpoint sim_play
+    {X1 X2} (q1: F1 X1) (q2: F2 X2) (re: r E1 E2)
+    (rf: r F1 F2) (p1: play E1 F1 X1) (s2: t E2 F2 X2): Prop :=
+    match p1 with
+    | pr r1 => exists r2, at_final s2 r2 /\ match_answ rf q1 q2 r1 r2
+    | prq X1' r1 q1' p_next =>
+        exists r2, at_final s2 r2 /\ match_answ rf q1 q2 r1 r2 /\
+        forall X2' (q2': F2 X2'),
+        match_ques (r_next rf q1 q2 r1 r2) q1' q2' ->
+        sim_play q1' q2' re (r_next rf q1 q2 r1 r2) p_next (after_final s2 r2 q2')
+    | pm Y1 m1 => exists Y2 (m2: E2 Y2), at_external s2 m2 /\ match_ques re m1 m2
+    | pmn Y1 m1 n1 p_next =>
+        exists Y2 (m2: E2 Y2), at_external s2 m2 /\ match_ques re m1 m2 /\
+        forall n2, match_answ re m1 m2 n1 n2 ->
+        sim_play q1 q2 (r_next re m1 m2 n1 n2) rf p_next (after_external s2 m2 n2)
+    end.
 
-  Inductive sim_s (re: r E1 E2) (rf: r F1 F2)
+  Definition sim_t
+    {X1 X2} (q1: F1 X1) (q2: F2 X2) (re: r E1 E2)
+    (rf: r F1 F2) (s1: t E1 F1 X1) (s2: t E2 F2 X2): Prop :=
+    forall p1, down p1 [= s1 -> sim_play q1 q2 re rf p1 s2.
+
+  (* Inductive sim_t: *)
+  (*   forall {X1 X2}, F1 X1 -> F2 X2 -> r E1 E2 -> r F1 F2 -> t E1 F1 X1 -> t E2 F2 X2 -> Prop := *)
+  (* | sim_t_intro X1 X2 (q1: F1 X1) (q2: F2 X2) re rf p1 p2 *)
+  (*     (match_final: *)
+  (*       forall r1, at_final p1 r1 -> *)
+  (*       exists r2, at_final p2 r2 /\ match_answ rf q1 q2 r1 r2 /\ *)
+  (*       forall {X1' X2'} (q1': F1 X1') (q2': F2 X2'), *)
+  (*         match_ques (r_next rf q1 q2 r1 r2) q1' q2' -> *)
+  (*       forall p1', after_final p1 r1 q1' p1' -> *)
+  (*       exists p2', after_final p2 r2 q2' p2' /\ *)
+  (*         sim_t q1' q2' re (r_next rf q1 q2 r1 r2) p1' p2') *)
+  (*     (match_external: *)
+  (*       forall {Y1} (m1: E1 Y1), at_external p1 m1 -> *)
+  (*       exists {Y2} (m2: E2 Y2), at_external p2 m2 /\ match_ques re m1 m2 /\ *)
+  (*       forall n1 n2, match_answ re m1 m2 n1 n2 -> *)
+  (*       forall p1', after_external p1 m1 n1 p1' -> *)
+  (*       exists p2', after_external p2 m2 n2 p2' /\ *)
+  (*         sim_t q1 q2 (r_next re m1 m2 n1 n2) rf p1' p2'): *)
+  (*   sim_t q1 q2 re rf p1 p2. *)
+
+  Definition sim_s (re: r E1 E2) (rf: r F1 F2)
     (s1: s E1 F1) (s2: s E2 F2) : Prop :=
-  | sim_s_intro
-    (match_initial:
-      forall {X1 X2} (mf1: F1 X1) (mf2: F2 X2),
-        match_ques rf mf1 mf2 ->
-      forall p1, initial_state s1 mf1 p1 ->
-      exists p2, initial_state s2 mf2 p2 /\
-      sim_p mf1 mf2 rf sim_s re p1 p2):
-    sim_s re rf s1 s2.
+    forall {X1 X2} (qf1: F1 X1) (qf2: F2 X2), match_ques rf qf1 qf2 ->
+    sim_t qf1 qf2 re rf (s1 _ qf1) (s2 _ qf2).
+
+  Instance sim_play_propers {re rf X1 X2} (q1: F1 X1) (q2: F2 X2):
+    Proper (play_ref --> ref ==> impl) (sim_play q1 q2 re rf).
+  Proof.
+    intros p1 p2 Hp. intros t1 t2 Ht. intros H.
+    unfold flip in Hp.
+    revert X2 t1 t2 Ht q1 q2 re rf H.
+    induction Hp; intros.
+    - destruct H as (r2 & Hf & Hr). exists r2. split; eauto.
+      unfold at_final in *.
+      etransitivity; eauto.
+    - destruct H as (r2 & Hf & Hr & Hnext). exists r2. split; eauto.
+      unfold at_final in *.
+      etransitivity; eauto.
+    - destruct H as (r2 & Hf & Hr & Hnext).
+      exists r2. split. unfold at_final in *; eauto.
+      etransitivity; eauto.
+      split; eauto.
+      intros. eapply IHHp. 2: apply Hnext; eauto.
+      unfold after_final.
+      apply sup_iff. intros (i & Hi). cbn.
+      eapply (fsup_at i). etransitivity; eauto. reflexivity.
+    - destruct H as (A2 & m2 & He & Hm).
+      eexists _, m2. split; eauto.
+      unfold at_external in *. etransitivity; eauto.
+    - destruct H as (A2 & m2 & He & Hm & Hnext).
+      eexists _, m2. split; eauto.
+      unfold at_external in *. etransitivity; eauto.
+    - destruct H as (A2 & m2 & He & Hm & Hnext).
+      eexists _, m2. split. unfold at_external in *.
+      etransitivity; eauto.
+      split; eauto.
+      intros. eapply IHHp. 2: apply Hnext; eauto.
+      unfold after_external.
+      apply sup_iff. intros (i & Hi). cbn.
+      eapply (fsup_at i). etransitivity; eauto. reflexivity.
+  Qed.
+
+  Instance sim_propers {re rf}:
+    Proper (ref --> ref ==> impl) (sim_s re rf).
+  Proof.
+    intros s1 s2 Hs. intros t1 t2 Ht. unfold flip in Hs.
+    intros Hp. unfold sim_s. intros * Hq.
+    specialize (Hp _ _ _ _ Hq). clear Hq.
+    unfold sim_t in *. intros p1 Hp1.
+    specialize (Hs X1 qf1).
+    eapply sim_play_propers.
+    - reflexivity.
+    - apply Ht.
+    - apply Hp. etransitivity; eauto.
+  Qed.
 
 End SIM.
 
 Generalizable All Variables.
 
 Section HCOMP.
+
+  Lemma map_prq_elim A A' `(s: t E F A')
+    (p: play E F A) (r: A) (q: F A'):
+    down p [= Downset.map (fun p => prq r q p) s ->
+    exists next, p [= prq r q next /\ down next [= s.
+  Proof.
+    intros Hp. unfold Downset.map in Hp.
+    pose proof (Downset.emb_join_dense s).
+    rewrite H in Hp. clear H.
+    setoid_rewrite Sup.mor in Hp.
+    apply Downset.emb_join_prime in Hp.
+    destruct Hp as ((i & Hi) & Hp). cbn in Hp.
+    setoid_rewrite @Downset.ext_ana in Hp. 2: admit.
+    apply (iff_sym (Downset.emb_mor _ _)) in Hp.
+    exists i. split; eauto.
+  Admitted.
+
+  Lemma map_pmn_elim A B `(s: t E F A)
+    (p: play E F A) (m: E B) (n: B):
+    down p [= Downset.map (fun p => pmn m n p) s ->
+    exists next, p [= pmn m n next /\ down next [= s.
+  Proof.
+    intros Hp. unfold Downset.map in Hp.
+    pose proof (Downset.emb_join_dense s).
+    rewrite H in Hp. clear H.
+    setoid_rewrite Sup.mor in Hp. 
+    apply Downset.emb_join_prime in Hp.
+    destruct Hp as ((i & Hi) & Hp). cbn in Hp.
+    setoid_rewrite @Downset.ext_ana in Hp. 2: admit.
+    apply (iff_sym (Downset.emb_mor _ _)) in Hp.
+    exists i. split; eauto.
+  Admitted.
+
+  Lemma at_final_intro_t `(t1: t F G A) `(t2: s E F) r:
+    at_final t1 r -> at_final (compose_t1 t1 t2) r.
+  Proof.
+    unfold at_final, compose_t1. intros Hp.
+    rewrite <- Hp. rewrite @Downset.ext_ana. 2: admit.
+    cbn. reflexivity.
+  Admitted.
+
+  Lemma after_final_compose_t
+    `(t1: t F G X) `(t2: s E F) r1 `(q2: G X'):
+    after_final (compose_t1 t1 t2) r1 q2 =
+      (compose_t1 (after_final t1 r1 q2) t2).
+  Proof.
+    unfold after_final, compose_t1.
+    unfold fsup.
+    setoid_rewrite Sup.mor.
+    apply antisymmetry.
+    - apply sup_iff. intros (i & Hi). cbn.
+  Admitted.
+
+  Lemma at_external_compose_t `(p: t F G A) {E X Y} (s: s E F) (m0: F X) (m: E Y):
+    at_external (s X m0) m ->
+    at_external p m0 ->
+    at_external (compose_t1 p s) m.
+  Proof.
+    unfold at_external, compose_t1.
+    intros Hp1 Hp2.
+    rewrite <- Hp2. rewrite @Downset.ext_ana. 2: admit. cbn.
+    unfold compose_t2. rewrite <- Hp1.
+    rewrite @Downset.ext_ana. 2: admit. cbn. reflexivity.
+  Admitted.
+
+  Definition filter_m `(p: t F G A): t F G A :=
+    sup { p' | (exists B (m: F B), pm m [= p') /\ down p' [= p }, down p'.
+
+  Lemma filter_m_at_external `(p: t E F A) `(m: E B):
+    at_external p m ->
+    at_external (filter_m p) m.
+  Proof.
+    unfold at_external, filter_m.
+    intros. apply (fsup_at (pm m)); try easy.
+    split; eauto. eexists _, m. easy.
+  Qed.
+
+  Lemma filter_m_after_external `(p: t E F A) `(m: E B) n:
+    after_external p m n =
+    after_external (filter_m p) m n.
+  Proof.
+    unfold after_external, filter_m.
+    apply antisymmetry.
+    - apply sup_iff. intros (x & Hx). cbn.
+      apply (fsup_at x); try easy.
+      apply (fsup_at (pmn m n x)); try easy.
+      split; eauto. eexists _, m. constructor.
+    - apply sup_iff. intros (x & Hx). cbn.
+      apply (fsup_at x); try easy.
+      apply Downset.emb_join_prime in Hx as ((i & Hi) & Hk).
+      cbn in Hk. destruct Hi.
+      etransitivity; eauto.
+  Qed.
+
+  Lemma after_external_compose_t `(p: t F G A) {E X} (s: s E F) (m: E X) n:
+    compose_t1 (filter_m p) (fun Y q => after_external (s _ q) m n) [=
+    after_external (compose_t1 p s) m n.
+  Proof.
+    unfold compose_t1 at 1, filter_m.
+    setoid_rewrite Sup.mor. apply sup_iff.
+    intros (i & Ha & Hb). cbn. rewrite @Downset.ext_ana. 2: admit.
+    destruct Ha as (? & q & Hq).
+    pose proof (Downset.emb_join_dense (compose_play1 (fun (Y : Type) (q0 : F Y) => after_external (s Y q0) m n) i)) as Hp.
+    rewrite Hp. apply sup_iff. intros (k & Hk). cbn.
+    unfold after_external.
+    apply (fsup_at k). 2: reflexivity.
+    unfold compose_t1.
+    rewrite <- Hb. rewrite @Downset.ext_ana. 2: admit. cbn.
+    inv Hq; subst_dep; cbn.
+    - cbn in Hk. unfold compose_t2 in Hk.
+      setoid_rewrite Sup.mor in Hk.
+      apply Downset.emb_join_prime in Hk as ((i & Hi) & Hk).
+      rewrite @Downset.ext_ana in Hk. 2: admit. cbn in Hk.
+      unfold compose_t2. rewrite <- Hi.
+      rewrite @Downset.ext_ana. 2: admit. cbn.
+      unfold Downset.map. rewrite <- Hk.
+      rewrite @Downset.ext_ana. 2: admit. reflexivity.
+    - cbn in Hk. unfold compose_t2 in Hk.
+      setoid_rewrite Sup.mor in Hk.
+      apply Downset.emb_join_prime in Hk as ((i & Hi) & Hk).
+      rewrite @Downset.ext_ana in Hk. 2: admit. cbn in Hk.
+      unfold compose_t2. rewrite <- Hi.
+      rewrite @Downset.ext_ana. 2: admit. cbn.
+      unfold Downset.map. rewrite <- Hk.
+      rewrite @Downset.ext_ana. 2: admit. reflexivity.
+  Admitted.
+
+  Lemma at_final_compose2 `(t1: t F G A) `(t2: s E F) `(m: F B) n r:
+    at_final (after_external t1 m n) r ->
+    at_final (t2 _ m) n ->
+    at_final (compose_t1 t1 t2) r.
+  Proof.
+    intros H1 H2. unfold at_final, after_external in *.
+    apply Downset.emb_join_prime in H1.
+    destruct H1 as ((i & Hi) & Hp). cbn in Hp.
+    apply (iff_sym (Downset.emb_mor _ _)) in Hp.
+    unfold compose_t1. rewrite <- Hi.
+    rewrite @Downset.ext_ana. 2: admit. cbn.
+    unfold compose_t2. rewrite <- H2.
+    rewrite @Downset.ext_ana. 2: admit. cbn.
+    assert (Hn: n = n) by reflexivity.
+    apply (sup_at Hn).
+    inv Hp; cbn. reflexivity.
+  Admitted.
+
+  Definition filter_r `(p: t F G A): t F G A :=
+    sup { p' | (exists r, pr r [= p') /\ down p' [= p }, down p'.
+
+  Lemma after_external_compose_t2 `(p: t F G A) `(t2: s E F) `(m1: F B) n1:
+    at_final (t2 _ m1) n1 ->
+    compose_t1 (after_external p m1 n1)
+      (fun X (m2 : F X) => after_final (t2 _ m1) n1 m2) [= compose_t1 p t2.
+  Proof.
+    assert (filter_r (t2 _ m1) [= t2 _ m1) as Ht2.
+    { unfold filter_r. apply sup_iff. intros (i & Hi). cbn. apply Hi. }
+    intros Hf. unfold compose_t1 at 1.
+    unfold after_external.
+    setoid_rewrite Sup.mor. apply sup_iff. intros (i & Hi). cbn.
+    rewrite @Downset.ext_ana. 2: admit.
+    unfold compose_t1. rewrite <- Hi. clear Hi.
+    rewrite @Downset.ext_ana. 2: admit.
+    cbn. unfold compose_t2. rewrite <- Ht2.  clear Ht2.
+    clear p. induction i.
+    - cbn. unfold filter_r.
+      rewrite fsup_mor. eapply (fsup_at (pr n1)).
+      split. exists n1. reflexivity. apply Hf.
+      rewrite @Downset.ext_ana. 2: admit.
+      cbn. eapply sup_at. reflexivity. reflexivity.
+    - cbn. unfold Downset.map. rewrite IHi. clear IHi.
+      rewrite @Downset.ext_ext. 2-3: admit.
+      unfold filter_r.
+      setoid_rewrite Sup.mor.
+      apply sup_iff. intros (x & Hx). apply (sup_at (exist _ x Hx)).
+      cbn. rewrite !@Downset.ext_ana. 2-3: admit.
+      destruct Hx as ((r & Hr) & Hb). inv Hr.
+      + cbn.
+        rewrite Sup.mor. apply sup_iff. intros <-.
+        eapply sup_at. reflexivity. reflexivity.
+      + cbn.
+        rewrite Sup.mor. apply sup_iff. intros <-.
+        eapply sup_at. reflexivity. reflexivity.
+    - cbn. unfold after_final.
+      unfold compose_t2.
+      rewrite fsup_mor. apply sup_iff.
+      intros (x & Hx). cbn.
+      rewrite @Downset.ext_ana. 2: admit.
+      unfold filter_r.
+      rewrite fsup_mor. eapply (fsup_at (prq n1 e x)).
+      split. exists n1. constructor. apply Hx.
+      rewrite @Downset.ext_ana. 2: admit.
+      cbn. eapply sup_at. reflexivity.
+      unfold compose_play2_obligation_1.
+      rewrite Sup.mor. eapply sup_at. Unshelve. 2: reflexivity.
+      unfold eq_rect. rewrite Sup.mor. eapply sup_at.
+      reflexivity.
+      rewrite @Downset.ext_ana. 2: admit.
+      reflexivity.
+    - cbn. unfold after_final.
+      unfold compose_t2.
+      rewrite fsup_mor. apply sup_iff.
+      intros (x & Hx). cbn.
+      rewrite @Downset.ext_ana. 2: admit.
+      unfold filter_r.
+      rewrite fsup_mor. eapply (fsup_at (prq n1 e x)).
+      split. exists n1. constructor. apply Hx.
+      rewrite @Downset.ext_ana. 2: admit.
+      cbn. eapply sup_at. reflexivity.
+      unfold compose_play2_obligation_1.
+      rewrite Sup.mor. eapply sup_at. Unshelve. 2: reflexivity.
+      unfold eq_rect. rewrite Sup.mor. eapply sup_at.
+      reflexivity.
+      rewrite @Downset.ext_ana. 2: admit.
+      reflexivity.
+  Admitted.
+
   Context `(s1: s F1 G1) `(s2: s E1 F1) `(t1: s F2 G2) `(t2: s E2 F2)
     (re: r E1 E2) (rf: r F1 F2) (rg: r G1 G2)
     (sim1: sim_s rf rg s1 t1) (sim2: sim_s re rf s2 t2).
 
   Theorem hcomp: sim_s re rg (compose s1 s2) (compose t1 t2).
   Proof.
-    constructor. intros * Hq * Hi.
-    unfold initial_state in Hi. cbn in Hi.
+    unfold sim_s. intros X1 X2 qg1 qg2 Hqg.
+    specialize (sim1 _ _ qg1 qg2 Hqg).
+    intros p1 Hp1. cbn in p1.
+    unfold compose in Hp1. unfold compose_t1 in Hp1.
+    pose proof (Downset.emb_join_dense (s1 X1 qg1)).
+    rewrite H in Hp1. setoid_rewrite Sup.mor in Hp1.
+    apply Downset.emb_join_prime in Hp1.
+    destruct Hp1 as ((c & Hc) & Hp1). cbn in Hp1.
+    rewrite @Downset.ext_ana in Hp1. 2: admit.
+    unfold sim_t in sim1. specialize (sim1 _ Hc).
+    clear H. clear Hc.
+    (* we could also induction on p1? *)
+    revert rf  sim1 re t2 sim2.
+    unfold compose. generalize (t1 X2 qg2).
+    revert X2 qg2 qg1 rg Hqg s2 Hp1.
+    induction c.
+    - intros. cbn in sim1. cbn in Hp1.
+      apply (iff_sym (Downset.emb_mor _ _)) in Hp1.
+      inv Hp1. cbn.
+      destruct sim1 as (r2 & Hf2 & Hr2).
+      exists r2. split; eauto.
+      apply at_final_intro_t. eauto.
+    - intros.
+      cbn in sim1. destruct sim1 as (r2 & Hf2 & Hr2 & Hnext).
+      clear sim1. cbn in Hp1.
+      apply map_prq_elim in Hp1 as (_next & Hp1 & Hpnext).
+      inv Hp1.
+      + subst_dep. cbn.
+        exists r2. split; eauto.
+        apply at_final_intro_t. eauto.
+      + subst_dep. cbn.
+        exists r2. split. apply at_final_intro_t. eauto.
+        split. eauto.
+        intros X2' q2' Hq2.
+        specialize (Hnext _ _ Hq2).
+        rewrite after_final_compose_t.
+        exploit (IHc next0). apply Hq2. 2: apply Hnext. 2: apply sim2.
+        etransitivity; eauto. apply Downset.emb_mor; eauto.
+        tauto.
+    - intros. cbn in sim1.
+      destruct sim1 as (Y1 & m1 & He1 & Hm1). clear sim1.
+      cbn in Hp1.
+      unfold sim_s in sim2. specialize (sim2 _ _ _ _ Hm1).
+      unfold compose_t2 in Hp1.
+      pose proof (Downset.emb_join_dense (s2 B e)).
+      rewrite H in Hp1. setoid_rewrite Sup.mor in Hp1.
+      apply Downset.emb_join_prime in Hp1.
+      destruct Hp1 as ((c & Hc) & Hp1). cbn in Hp1.
+      rewrite @Downset.ext_ana in Hp1. 2: admit.
+      specialize (sim2 _ Hc).
+      clear Hc Hqg H Hm1. revert t2 p1 re sim2 Hp1.
+      revert p He1.
+      induction c; intros.
+      + cbn in Hp1. apply bot_elim in Hp1. inv Hp1.
+      + cbn in Hp1. apply bot_elim in Hp1. inv Hp1.
+      + cbn in Hp1. apply (iff_sym (Downset.emb_mor _ _)) in Hp1.
+        inv Hp1. subst_dep. cbn.
+        cbn in sim2. destruct sim2 as (Y2 & m2 & He2 & Hm2).
+        exists Y2, m2. split; eauto.
+        eapply at_external_compose_t; eauto.
+      + cbn in Hp1. apply map_pmn_elim in Hp1 as (_next & Hp1 & Hpnext).
+        inv Hp1.
+        * subst_dep. cbn in sim2.
+          destruct sim2 as (Y2 & m2 & He2 & Hm2 & ?). clear sim2.
+          exists Y2, m2. split; eauto.
+          eapply at_external_compose_t; eauto.
+        * subst_dep. cbn in sim2.
+          destruct sim2 as (Y2 & m2 & He2 & Hm2 & Hnext2). clear sim2.
+          cbn. exists Y2, m2. split; eauto.
+          eapply at_external_compose_t; eauto.
+          split. apply Hm2.
+          intros n2 Hn2. specialize (Hnext2 _ Hn2).
+          set (next_t2 := fun A q => after_external (t2 A q) m2 n2).
+          assert (He3: at_external (filter_m p) m1).
+          apply filter_m_at_external. eauto.
+          specialize (IHc e (filter_m p) He3 next_t2).
+          (* TODO: rewrite *)
+          eapply sim_play_propers. reflexivity. apply after_external_compose_t.
+          apply IHc. apply Hnext2.
+          etransitivity; eauto. apply Downset.emb_mor. eauto.
+    - intros. cbn in sim1.
+      destruct sim1 as (Y1 & m1 & He1 & Hm1 & Hnext1). clear sim1.
+      unfold sim_s in sim2. specialize (sim2 _ _ _ _ Hm1).
+      cbn in Hp1. unfold compose_t2 in Hp1.
+      pose proof (Downset.emb_join_dense (s2 B e)).
+      rewrite H in Hp1. setoid_rewrite Sup.mor in Hp1. 
+      apply Downset.emb_join_prime in Hp1.
+      destruct Hp1 as ((d & Hd) & Hp1). cbn in Hp1.
+      rewrite @Downset.ext_ana in Hp1. 2: admit.
+      specialize (sim2 _ Hd). clear Hd. clear H.
+      revert p1 b Hp1 t2 re sim2 Hnext1.
+      revert p He1.
+      (* induction on s2's behavior *)
+      induction d; intros.
+      + (* s1 calls s2, and s2 returns and terminates with no further states. *)
+        cbn in Hp1.
+        apply Downset.emb_join_prime in Hp1.
+        destruct Hp1 as (Hb & Hp1). subst.
+        cbn in sim2. destruct sim2 as (r2 & Hf2 & Hr2).
+        clear sim2. specialize (Hnext1 _ Hr2).
+        specialize (IHc p1 _ _ _ _ Hqg _ Hp1 _ _ Hnext1).
+        exploit IHc.
+        { unfold sim_s. intros. unfold sim_t. intros.
+          apply bot_elim in H0. inv H0. }
+        intros HX.
+        (* My guess is compose_t1 (after_external p m1 r2) ?Goal6 = compose_t1 p t2 *)
+        eapply sim_play_propers. reflexivity.
+        apply after_external_compose_t2. apply Hf2. apply HX.
+      + (* s1 calls s2, and s2 returns, and the execution goes on. *)
+        cbn in Hp1.
+        apply Downset.emb_join_prime in Hp1.
+        destruct Hp1 as (Hb & Hp1). subst.
+        cbn in sim2. destruct sim2 as (r2 & Hf2 & Hr2 & Hnext2).
+        clear sim2. specialize (Hnext1 _ Hr2).
+        unfold compose_play2_obligation_1 in Hp1.
+        specialize (IHc p1 _ _ _ _ Hqg _ Hp1 _ _ Hnext1).
+        exploit IHc.
+        {
+          unfold sim_s. intros * Hq.
+          unfold sim_t. intros * Hp0.
+          apply Downset.emb_join_prime in Hp0.
+          destruct Hp0 as (HA & Hp0). subst.
+          unfold eq_rect in Hp0.
+          apply Downset.emb_join_prime in Hp0.
+          destruct Hp0 as (Hf & Hp0). subst.
+          apply (iff_sym (Downset.emb_mor _ _)) in Hp0.
+          (* TODO: rewrite not work.. *)
+          eapply sim_play_propers. apply Hp0. reflexivity.
+          apply Hnext2. apply Hq.
+        }
+        intros HX.
+        eapply sim_play_propers. reflexivity.
+        apply after_external_compose_t2. apply Hf2. apply HX.
+      + cbn in Hp1. apply (iff_sym (Downset.emb_mor _ _)) in Hp1.
+        inv Hp1. subst_dep. cbn.
+        cbn in sim2. destruct sim2 as (Y2 & m2 & He2 & Hm2).
+        exists Y2, m2. split; eauto. eapply at_external_compose_t; eauto.
+      + cbn in Hp1.
+        apply map_pmn_elim in Hp1 as (next_ & Hp1 & Hpnext).
+        destruct sim2 as (Y2 & m2 & He2 & Hm2 & Hnext2). clear sim2.
+        inv Hp1.
+        * subst_dep. cbn. exists Y2, m2. split; eauto.
+          eapply at_external_compose_t; eauto.
+        * subst_dep. cbn. exists Y2, m2.
+          split. eapply at_external_compose_t; eauto.
+          split. eauto.
+          intros n2 Hn2. specialize (Hnext2 _ Hn2).
+          eapply sim_play_propers. reflexivity. apply after_external_compose_t.
+          specialize (IHd _ Hm1).
+          assert (He3: at_external (filter_m p) m1).
+          apply filter_m_at_external. eauto.
+          specialize (IHd _ He3).
+          specialize (IHd _ _ Hpnext).
+          (* TODO: rewrite not work.. *)
+          eapply sim_play_propers. apply H1. reflexivity.
+          apply IHd. apply Hnext2.
+          intros n1 Hn1. rewrite <- filter_m_after_external.
+          apply Hnext1. eauto.
+  Admitted.
 
 End HCOMP.
+
